@prefix dct: <http://purl.org/dc/terms/> .
@prefix rdf: <http://www.w3.org/1999/02/22-rdf-syntax-ns#> .
@prefix rdfs: <http://www.w3.org/2000/01/rdf-schema#> .
@prefix skos: <http://www.w3.org/2004/02/skos/core#> .
@prefix skosxl: <http://www.w3.org/2008/05/skos-xl#> .
@prefix xml: <http://www.w3.org/XML/1998/namespace> .
@prefix xsd: <http://www.w3.org/2001/XMLSchema#> .
@prefix vann: <http://purl.org/vocab/vann/> .
@prefix vs: <http://www.w3.org/2003/06/sw-vocab-status/ns#> .
@prefix adms: <http://www.w3.org/ns/adms#> .
@prefix resourceType: <http://purl.org/dcx/lrmi-vocabs/learningResourceType/> .
@prefix bibo: <http://purl.org/ontology/bibo/status/> .

resourceType: a skos:ConceptScheme ;
    dct:title "LRMI Learning Resource Type Vocabulary"@en-US ;
    dct:creator "LRMI Task Group (DCMI)"@en-US ;
    dct:dateSubmitted "2015-01-21"^^xsd:date ;
    dct:description "A concept scheme defining the predominant genre, type or kind characterizing a learning resource"@en-US ;
    dct:source "Based in part on the CEDS Learning Resource Type vocabulary found at https://ceds.ed.gov/element/000928"@en-US ;
    skos:hasTopConcept resourceType:ActivityPlan, resourceType:Assessment, resourceType:AssessmentItem, resourceType:EducatorCurriculumGuide, resourceType:InteractiveLearningSoftware, resourceType:LessonPlan, resourceType:RecordedLesson, resourceType:RubricScoringGuide, resourceType:Textbook, resourceType:UnitPlan;
    adms:status bibo:draft .

resourceType:ActivityPlan a skos:Concept ;
    skos:prefLabel "Activity plan"@en-US ;
    skosxl:prefLabel resourceType:label-ActivityPlan ;
    skos:definition "A detailed description of an activity engaged in by the learner for the purpose of acquiring certain skills, concepts, or knowledge, whether guided by an instructor or not."@en-US ;
    skos:scopeNote "There may be several activities in a lesson or an activity may take place outside of a lesson.";
    skos:inScheme resourceType: ;
    dct:source "Based on Common Education Data Standards (CEDS): https://ceds.ed.gov/element/000928/#LearningActivity"@en-US ;
    vs:term_status "unstable" .

resourceType:Assessment a skos:Concept ;
    skos:prefLabel "Assessment"@en-US ;
    skosxl:prefLabel resourceType:label-alternateAssessment ;
    skos:definition " A set of assessment items used to evaluate or promote learning."@en-US ;
    skos:inScheme resourceType: ;
    dct:source "Based on Common Education Data Standards (CEDS): https://ceds.ed.gov/element/000928/#Assessment"@en-US ;
    vs:term_status "unstable" .

resourceType:AssessmentItem a skos:Concept ;
    skos:prefLabel "Assessment item"@en-US ;
    skosxl:prefLabel resourceType:label-assessmentItem ; 
    skos:definition "A specific prompt, that defines a question or protocol for a measurable activity that triggers a response from a person used to determine whether the person has mastered a learning objective."@en-US ;
    skos:inScheme resourceType: ;
    dct:source "Based on Common Education Data Standards (CEDS): https://ceds.ed.gov/element/000928#AssessmentItem"@en-US ;
    vs:term_status "unstable" .

resourceType:EducatorCurriculumGuide a skos:Concept ;
    skos:prefLabel "Educator/Curriculum guide"@en-US ;
    skosxl:prefLabel resourceType:label-EducatorCurriculumGuide ;
    skos:definition "A document that defines what concepts should be taught and/or how a concept should be taught effectively."@en-US ;
    skos:inScheme resourceType: ;
    dct:source "Based on Common Education Data Standards (CEDS): https://ceds.ed.gov/element/000928#EducatorCurriculumGuide"@en-US ;
    vs:term_status "unstable" .

resourceType:InteractiveLearningSoftware a skos:Concept ;
    skos:prefLabel "Interactive Learning Software/Application"@en-US ;
    skosxl:prefLabel resourceType:label-InteractiveLearningSoftware ;
    skos:definition "A software application that enable interactive learning activities."@en-US ;
    skos:inScheme resourceType: ;
    vs:term_status "unstable" .

resourceType:LessonPlan a skos:Concept ;
    skos:prefLabel "Lesson Plan"@en-US ;
    skosxl:prefLabel resourceType:label-LessonPlan ;
    skos:definition "A detailed description of the course of instruction for a Â­short period of time that is used by a teacher to guide class instruction. A Lesson may define one or more learning activities."@en-US ;
    skos:inScheme resourceType: ;
    dct:source "Based on Common Education Data Standards (CEDS): https://ceds.ed.gov/element/000928#Lesson"@en-US ;
    vs:term_status "unstable" .

resourceType:RecordedLesson a skos:Concept ;
    skos:prefLabel "Recorded lesson"@en-US ;
    skosxl:prefLabel resourceType:label-LessonPlan ;
    skos:definition "An audio or video recording, or a textual record (e.g. transcript or edited script) of a lesson, lecture or similar short instructional event."@en-US ;
    skos:scopeNote "Can be used in conjunction with properties such as dcterm:format or with a suitable schema.org Type in order to indicate whether the recording is audio, video or text."@en-us ;
    skos:inScheme resourceType: ;
    vs:term_status "unstable" .

resourceType:RubricScoringGuide a skos:Concept ;
    skos:prefLabel "Rubric/Scoring guide"@en-US ;
    skosxl:prefLabel resourceType:label-RubricScoringGuide ;
    skos:definition "A document or guide that is used to delineate consistent criteria for example in various forms of assessment and evaluation."@en-US ;
    skos:inScheme resourceType: ;
    dct:source "Based on Common Education Data Standards (CEDS): https://ceds.ed.gov/element/000928#RubricScoringGuide"@en-US ;
    vs:term_status "unstable" .

resourceType:Textbook a skos:Concept ;
    skos:prefLabel "Textbook"@en-US ;
    skosxl:prefLabel resourceType:label-Textbook ;
    skos:definition "A book used as a standard source of information on a particular subject."@en-US ;
    skos:inScheme resourceType: ;
    dct:source "Based on Common Education Data Standards (CEDS): https://ceds.ed.gov/element/000928#Textbook"@en-US ;
    vs:term_status "unstable" .

resourceType:UnitPlan a skos:Concept ;
    skos:prefLabel "Unit Plan"@en-US ;
    skosxl:prefLabel resourceType:label-UnitPlan ;
    skos:definition "A long-range plan of instruction on a particular concept."@en-US ;
    skos:scopeNote "A Unit contains several lessons, activities and or assessments that are related."@en-US ;
    skos:inScheme resourceType: ;
    dct:source "Based on Common Education Data Standards (CEDS): https://ceds.ed.gov/element/000928/#Unit"@en-us ;
    vs:term_status "unstable" .
    
#=============================
# EXTENDED LABELS
#=============================

resourceType:label-ActivityPlan a skosxl:label ;
    skosxl:literalForm "Activity plan"@en-US .

resourceType:label-Assessment a skosxl:label ;
    skosxl:literalForm "Assessment"@en-US .

resourceType:label-AssessmentItem a skosxl:label ;
    skosxl:literalForm "Assessment item"@en-US .

resourceType:label-EducatorCurriculumGuide a skosxl:label ;
    skosxl:literalForm "Educator/Curriculum guide"@en-US .

resourceType:label-InteractiveLearningSoftware a skosxl:label ;
    skosxl:literalForm "Interactive Learning Software/Applications"@en-US .

resourceType:label-LessonPlan a skosxl:label ;
    skosxl:literalForm "Lesson plan"@en-US .

resourceType:label-RecordedLesson a skosxl:label ;
    skosxl:literalForm "Recorded lesson"@en-US .

resourceType:label-RubricScoringGuide a skosxl:label ;
    skosxl:literalForm "Rubric/Scoring guide"@en-US .

resourceType:label-Textbook a skosxl:label ;
    skosxl:literalForm "Textbook"@en-US .

resourceType:label-UnitPlan a skosxl:label ;
    skosxl:literalForm "Unit Plan"@en-US .